theories/logrel/ftlr/ftlr_base.v
@@ -5,12 +5,12 @@ From cap_machine Require Export logrel.
 
 Section fundamental.
   Context
-    {Σ:gFunctors}
+    {Σ:gFunctors} {Cname : CmptNameG}
     {ceriseg:ceriseG Σ} {sealsg: sealStoreG Σ}
-    {Cname : CmptNameG}
-    {stsg : STSG Addr region_type Σ} {heapg : heapGS Σ}
-    {cstackg : CSTACKG Σ}
+    (* {stsg : STSG Addr region_type Σ} {heapg : heapGS Σ} *)
     {nainv: logrel_na_invs Σ}
+    {cinvg : cinvG Σ} {gstkg: gstacksIG Σ}
+    {cstackg : CSTACKG Σ}
     `{MP: MachineParameters}
   .
 
@@ -31,8 +31,9 @@ Section fundamental.
             full_map r_ih
             -∗ (∀ (r : RegName) v, ⌜r ≠ PC⌝ → ⌜r_ih !! r = Some v⌝ → interp W_ih C_ih v)
             -∗ registers_pointsto (<[PC:= WCap p_ih g_ih b_ih e_ih a_ih]> r_ih)
-            -∗ region W_ih C_ih
-            -∗ sts_full_world W_ih C_ih
+            (* -∗ region W_ih C_ih *)
+            (* -∗ sts_full_world W_ih C_ih *)
+            -∗ interp_world W_ih
             -∗ interp_continuation cstk Ws Cs
             -∗ ⌜frame_match Ws Cs cstk W_ih C_ih⌝
             -∗ na_own logrel_nais ⊤
@@ -42,7 +43,7 @@ Section fundamental.
 
   Definition ftlr_instr_base (W : WORLD) (C : CmptName) (regs : leibnizO Reg)
     (p p' : Perm) (g : Locality) (b e a : Addr)
-    (w : Word) (ρ : region_type) (P : V) (Pinstr : Prop) (cstk : CSTK) (Ws : list WORLD) (Cs : list CmptName)
+    (w : Word) (P : V) (Pinstr : Prop) (cstk : CSTK) (Ws : list WORLD) (Cs : list CmptName)
     : Prop :=
     validPCperm p g
     → (∀ x : RegName, is_Some (regs !! x))
@@ -51,34 +52,37 @@ Section fundamental.
     → PermFlowsTo p p'
     → isO p' = false
     → (persistent_cond P)
-    → (if isWL p then region_state_pwl W a else region_state_nwl W a g)
-    → std W !! a = Some ρ
-    → ρ ≠ Revoked
+    (* → (if isWL p then region_state_pwl W a else region_state_nwl W a g) *)
+    (* → std W !! a = Some ρ *)
+    (* → ρ ≠ Revoked *)
     → Pinstr
     -> ftlr_IH
     -∗ fixpoint interp1 W C (WCap p g b e a)
     -∗ (∀ (r : RegName) v, ⌜r ≠ PC⌝ → ⌜regs !! r = Some v⌝ → interp W C v)
-    -∗ rel C a p' (safeC P)
+    (* -∗ rel C a p' (safeC P) *)
     -∗ □ (if decide (readAllowed_a_in_regs (<[PC:=WCap p g b e a]> regs) a)
             then ▷ (rcond P C p' interp)
             else emp)
     -∗ □ (if decide (writeAllowed_a_in_regs (<[PC:=(WCap p g b e a)]> regs) a)
           then ▷ wcond P C interp
           else emp)
-    -∗ monoReq W C a p' P
-    -∗ (▷ (if decide (ρ = Temporary)
-           then (if isWL p'
-                 then future_pub_mono C (safeC P) w
-                 else (if isDL p' then future_pub_mono C (safeC P) w else future_priv_mono C (safeC P) w))
-           else future_priv_mono C (safeC P) w))
+    -∗ interp_ref_inv W C p' g a P
+    -∗ future_mono C P
+    (* -∗ monoReq W C a p' P *)
+    (* -∗ (▷ (if decide (ρ = Temporary) *)
+    (*        then (if isWL p' *)
+    (*              then future_pub_mono C (safeC P) w *)
+    (*              else (if isDL p' then future_pub_mono C (safeC P) w else future_priv_mono C (safeC P) w)) *)
+    (*        else future_priv_mono C (safeC P) w)) *)
     -∗ ▷ P W C w
     -∗ interp_continuation cstk Ws Cs
     -∗ ⌜frame_match Ws Cs cstk W C⌝
-    -∗ sts_full_world W C
+    (* -∗ sts_full_world W C *)
     -∗ na_own logrel_nais ⊤
     -∗ cstack_frag cstk
-    -∗ open_region W C a
-    -∗ sts_state_std C a ρ
+    (* -∗ open_region W C a *)
+    -∗ interp_world W
+    (* -∗ sts_state_std C a ρ *)
     -∗ a ↦ₐ w
     -∗ PC ↦ᵣ (WCap p g b e a)
     -∗ ([∗ map] k↦y ∈ delete PC regs, k ↦ᵣ y)
@@ -89,8 +93,8 @@ Section fundamental.
 
   Definition ftlr_instr (W : WORLD) (C : CmptName) (regs : leibnizO Reg)
     (p p' : Perm) (g : Locality) (b e a : Addr)
-    (w : Word) (i: instr) (ρ : region_type) (P : V) (cstk : CSTK) (Ws : list WORLD) (Cs : list CmptName)
+    (w : Word) (i: instr) (P : V) (cstk : CSTK) (Ws : list WORLD) (Cs : list CmptName)
     : Prop :=
-    ftlr_instr_base W C regs p p' g b e a w ρ P (decodeInstrW w = i) cstk Ws Cs.
+    ftlr_instr_base W C regs p p' g b e a w P (decodeInstrW w = i) cstk Ws Cs.
 
 End fundamental.
